Final part of moving Program code inside the main code. Adapted add_definition/fixpoint and parsing of the "Program" prefix.
git-svn-id: svn+ssh://scm.gforge.inria.fr/svn/coq/trunk@15036 85f007b7-540e-0410-9357-904b9bb8a0f7

kernel/environ.ml
@@ -100,6 +100,7 @@ let map_named_val f (ctxt,ctxtv) =
 let empty_named_context = empty_named_context
 
 let push_named = push_named
+let push_named_context = List.fold_right push_named
 let push_named_context_val = push_named_context_val
 
 let val_of_named_context ctxt =
