plugins/subtac/subtac.mli
@@ -1,2 +1,0 @@
-val require_library : string -> unit
-val subtac : Pp.loc * Vernacexpr.vernac_expr -> unit
