toplevel/obligations.mli
@@ -1,10 +1,55 @@
+(************************************************************************)
+(*  v      *   The Coq Proof Assistant  /  The Coq Development Team     *)
+(* <O___,, *   INRIA - CNRS - LIX - LRI - PPS - Copyright 1999-2010     *)
+(*   \VV/  **************************************************************)
+(*    //   *      This file is distributed under the terms of the       *)
+(*         *       GNU Lesser General Public License Version 2.1        *)
+(************************************************************************)
+
+open Environ
+open Tacmach
+open Term
+open Evd
 open Names
 open Pp
 open Util
+open Tacinterp
 open Libnames
-open Evd
 open Proof_type
 open Vernacexpr
+open Decl_kinds
+open Tacexpr
+
+(** Forward declaration. *)
+val declare_fix_ref : (definition_object_kind -> identifier ->
+  constr -> types -> Impargs.manual_implicits -> global_reference) ref
+
+val declare_definition_ref :
+  (identifier -> locality * definition_object_kind ->
+     Entries.definition_entry -> Impargs.manual_implicits
+       -> global_reference declaration_hook -> global_reference) ref
+
+val non_instanciated_map : env -> evar_map ref -> evar_map -> evar_map
+
+val mkMetas : int -> constr list
+
+val evar_dependencies : evar_map -> int -> Intset.t
+val sort_dependencies : (int * evar_info * Intset.t) list -> (int * evar_info * Intset.t) list
+
+(* env, id, evars, number of function prototypes to try to clear from
+   evars contexts, object and type *)
+val eterm_obligations : env -> identifier -> evar_map -> evar_map -> int ->
+  ?status:obligation_definition_status -> constr -> types -> 
+  (identifier * types * hole_kind located * obligation_definition_status * Intset.t * 
+      tactic option) array
+    (* Existential key, obl. name, type as product, 
+       location of the original evar, associated tactic,
+       status and dependencies as indexes into the array *)
+  * ((existential_key * identifier) list * ((identifier -> constr) -> constr -> constr)) *
+    constr * types
+    (* Translations from existential identifiers to obligation identifiers 
+       and for terms with existentials to closed terms, given a 
+       translation from obligation identifiers to constrs, new term, new type *)
 
 type obligation_info =
   (identifier * Term.types * hole_kind located *
@@ -29,7 +74,7 @@ val add_definition : Names.identifier -> ?term:Term.constr -> Term.types ->
   ?kind:Decl_kinds.definition_kind ->
   ?tactic:Proof_type.tactic ->
   ?reduce:(Term.constr -> Term.constr) ->
-  ?hook:(Tacexpr.declaration_hook) -> obligation_info -> progress
+  ?hook:(unit Tacexpr.declaration_hook) -> obligation_info -> progress
 
 type notations = (Vernacexpr.lstring * Topconstr.constr_expr * Topconstr.scope_name option) list
 
@@ -43,7 +88,7 @@ val add_mutual_definitions :
   ?tactic:Proof_type.tactic ->
   ?kind:Decl_kinds.definition_kind ->
   ?reduce:(Term.constr -> Term.constr) ->
-  ?hook:Tacexpr.declaration_hook ->
+  ?hook:unit Tacexpr.declaration_hook ->
   notations ->
   fixpoint_kind -> unit
 
@@ -70,4 +115,3 @@ val admit_obligations : Names.identifier option -> unit
 exception NoObligations of Names.identifier option
 
 val explain_no_obligations : Names.identifier option -> Pp.std_ppcmds
-
